src/theories/monad_aux.v
@@ -1,4 +1,5 @@
 From ExtLib Require Import Structures.Monads.
+From stdpp Require Import vector.
 
 Module monad_option.
   
@@ -7,7 +8,7 @@ Module monad_option.
     refine {| ret t x := Some x;
               bind t u mt f := match mt with | None => None | Some t => f t end;
            |}.
-  Qed.
+  Defined.
 
   Fixpoint listFromSome {A : Type} (l : list (option A)) : list A :=
   match l with
@@ -19,7 +20,99 @@ Module monad_option.
     end
   end.
 
+  Definition boolCheckOption {A : Type} (b : bool) : option bool :=
+    match b with
+    | false => None
+    | true => Some true
+    end.
+
 End monad_option.
+
+Module monad_sum.
+  Instance MonadEither {E : Type} : Monad (sum E).
+  Proof.
+    refine {| ret t x := inr x;
+              bind t u mt f := match mt with | inl l => inl l | inr r => f r end;
+           |}.
+  Defined.
+  
+  Definition unpackOptionWithLeft {A B : Type} (v : option B) (err : A) : sum A B :=
+    match v with
+    | None => inl err
+    | Some v' => inr v'
+    end.
+End monad_sum.
+
+Fixpoint listBind {A B : Type} (l : list A) (f : A -> list B) : list B :=
+  match l with
+  | nil => nil
+  | cons x xs => app (f x) (listBind xs f)
+  end.
+
+Fixpoint listFmap {A B : Type} (f : A -> B) (l : list A) : list B :=
+  match l with
+  | nil => nil
+  | cons x xs => cons (f x) (listFmap f xs)
+  end.
+                     
+Instance MonadList : Monad list.
+Proof.
+  refine {| ret t x := cons x nil;
+            bind t u := listBind
+         |}.
+Defined.
+
+Module monad_list.
+  
+End monad_list.
+
+Module monad_general.
+  From stdpp Require Import listset_nodup.
+
+  Lemma sequenceMNoDup {A : Type} {M : Type -> Type} `{Monad M} (l : listset_nodup (M A)) : M (listset_nodup A).
+  Proof.
+    destruct l as [car prf].
+    induction car as [| x xs HQ].
+    - apply ret; apply empty.
+    - eapply bind.
+      + exact x.
+      + intros a.
+        eapply bind.
+        * apply HQ.
+          rewrite NoDup_ListNoDup in prf.
+          rewrite List.NoDup_cons_iff in prf.
+          destruct prf as [prf1 prf2].
+          rewrite <- NoDup_ListNoDup in prf2.
+          exact prf2.
+        * intros l'.
+          apply ret.
+          exact l'.
+    Defined.
+  
+  Fixpoint sequenceMList {A : Type} {M : Type -> Type} `{Monad M} (l : list (M A)) : M (list A) :=
+    match l with
+    | nil => ret nil
+    | cons x xs => bind x (fun x' => bind (sequenceMList xs) (fun xs' => ret (cons x' xs')))
+    end.
+  
+  Definition mapM {A B : Type} {M : Type -> Type} `{Monad M} (f : A -> M B) (l : list A) : M (list B) :=
+    sequenceMList (listFmap f l).
+
+  (* Generalize over traverseable *)
+  Fixpoint foldrMVec {A B : Type} {n : nat} {M : Type -> Type} `{Monad M}
+           (m : A -> B -> M B) (v : vec A n) (i : B) : M B :=
+    match v with
+    | vnil => ret i
+    | vcons x xs => bind (m x i) (foldrMVec m xs)
+    end.
+
+Fixpoint sequenceMVec {A : Type} {n : nat} {M : Type -> Type} `{Monad M} (v : vec (M A) n) : M (vec A n) :=
+  match v with
+  | vnil => ret vnil
+  | vcons x xs => bind x (fun x' => bind (sequenceMVec xs) (fun k => ret (vcons x' k)))
+  end.
+  
+End monad_general.
 
 Module monad_base_notation.
   
